\documentclass[a4paper,12pt]{article}

\usepackage{amsmath}
\usepackage{times}

\newcommand{\D}{\mathrm{d}}
\newcommand{\E}{\mathrm{e}}
\newcommand{\I}{\mathrm{i}}

\newcommand{\bA}{\boldsymbol{\alpha}}
\newcommand{\gnijk}[4]{g^{(#1)}_{#2,#3,#4}}
\newcommand{\gnbarijk}[4]{\overline{g}^{(#1)}_{#2,#3,#4}}

\begin{document}

From Cohl and Tohline:
\begin{align}
  \label{equ:basic}
  \frac{1}{R}
  &=
  \frac{1}{\pi\sqrt{rr_{1}}}
  \sum_{m=-\infty}^{\infty}
  \E^{\I m(\theta-\theta_{1})}
  Q_{m-1/2}(\chi),\\
  R^{2}
  &=
  r^{2} + r_{1}^{2} - 2rr_{1}\cos(\theta-\theta_{1}) +
  x^{2},\nonumber\\
  \chi
  &=
  \frac{r^{2} + r_{1}^{2} + x^{2}}{2rr_{1}}.
\end{align}

Field from an azimuthal mode:
\begin{align}
  \label{equ:gfunc}
  G
  &=
  \int_{0}^{2\pi}
  \frac{\E^{\I n\theta_{1}}}{4\pi R}\,\D \theta_{1},\\
  &=
  \E^{\I n\theta}G_{n},\\
  G_{n}
  &=
  \frac{Q_{n-1/2}(\chi)}{2\pi\sqrt{rr_{1}}}. 
\end{align}

Recursion (Cohl and Tohline)
\begin{align}
  \label{equ:recursion}
  G_{0}
  &=
  \frac{1}{2\pi}\frac{\mu}{\sqrt{rr_{1}}}K(\mu),\\
  G_{1}
  &=
  \frac{1}{2\pi}\frac{}{\sqrt{rr_{1}}}
  \left(
    \chi\mu K(\mu) - (\chi+1)\mu E(\mu)
  \right),\\
  G_{n}
  &=
  4\frac{n-1}{2n-1}\chi G_{n-1} - \frac{2n-3}{2n-1}G_{n-2},\\
  (2n-3)G_{n-2}
  &=
  4(n-1)\chi G_{n-1} - (2n-1)G_{n}.
\end{align}
(The descending recursion to find $G_{n}$ is stable.)

Derivative w.r.t. $x$. From G\&R,~8.832,
\begin{align}
  \label{equ:gfunc:dx}
  \frac{\partial G_{n}}{\partial x}
  &=
  (n+1/2)
  \left(G_{n+1} - \chi G_{n}\right)
  \frac{1}{\chi^{2}-1}\frac{\partial\chi}{\partial x},\\
  &= \frac{(n-1/2)(n+1/2)}{2n}
  \left(G_{n+1} - G_{n-1}\right)
  \frac{1}{\chi^{2}-1}\frac{\partial\chi}{\partial x},\\
  \frac{1}{\chi^{2}-1}\frac{\partial\chi}{\partial x}
  &=
  \frac{x}{rr_{1}}\frac{1}{\chi-1}\frac{1}{\chi+1}.\\
  \frac{\partial G_{0}}{\partial x}
  &=
  -\frac{x}{8\pi}\frac{1}{(rr_{1})^{3/2}}\frac{\mu^{3}}{1-\mu^{2}}E(\mu).
\end{align}

Derivative w.r.t. $r_{1}$. From G\&R,~8.832,
\begin{align}
  \label{equ:gfunc:dx}
  \frac{\partial G_{n}}{\partial r_{1}}
  &=
  -\frac{G_{n}}{2r_{1}}
  +
  (n+1/2)
  \left(G_{n+1} - \chi G_{n}\right)
  \frac{1}{\chi^{2}-1}\frac{\partial\chi}{\partial r_{1}},\\
  % &= \frac{(n-1/2)(n+1/2)}{2n}
  % \left(G_{n+1} - G_{n-1}\right)
  % \frac{1}{\chi^{2}-1}\frac{\partial\chi}{\partial x},\\
  % \frac{1}{\chi^{2}-1}\frac{\partial\chi}{\partial x}
  % &=
  % \frac{x}{rr_{1}}\frac{1}{\chi-1}\frac{1}{\chi+1}.\\
  % \frac{\partial G_{0}}{\partial x}
  % &=
  % -\frac{x}{8\pi}\frac{1}{(rr_{1})^{3/2}}\frac{\mu^{3}}{1-\mu^{2}}E(\mu).
\end{align}

Derivatives of $f=1/(\chi\pm1)$,
\begin{align*}
  f = \frac{1}{\chi\pm1} &= \frac{2rr_{1}}{(r\pm r_{1})^{2} + x^{2}},\\
  \left[
    (r\pm r_{1})^{2} + x^{2}
  \right]f
  &=
  2rr_{1},\\
  \frac{\partial^{m}}{\partial x^{m}}
  \left[
    (r\pm r_{1})^{2} + x^{2}
  \right]f &=
  \sum_{q=0}^{m}
  \binom{m}{q}
  \frac{\partial^{q}}{\partial x^{q}}
  \left[
    (r\pm r_{1})^{2} + x^{2}
  \right]
  \frac{\partial^{m-q}f}{\partial x^{m-q}}
  =
  %\frac{\partial}{\partial}
  0,\\
  \frac{\partial^{m}f}{\partial x^{m}}
  &=
  -
  \sum_{q=1}^{m}
  \binom{m}{q}
  \frac{\partial^{q}}{\partial x^{q}}
  \left[
    (r\pm r_{1})^{2} + x^{2}
  \right]
  \frac{\partial^{m-q}f}{\partial x^{m-q}},\\
  &= -\frac{m}{2rr_{1}}
  \left[
    2x
    \frac{\partial^{m-1}f}{\partial x^{m-1}}
    + (m-1)
    \frac{\partial^{m-2}f}{\partial x^{m-2}}
  \right]f,\quad m\geq 2,\\
  \frac{\partial f}{\partial x}
  &=
  -\frac{x}{rr_{1}}f^{2}. 
\end{align*}

Derivatives of $f=1/(\chi^{2}-1)$:
\begin{align*}
  \rho_{\pm}^{2} &= (r\pm r_{1})^{2} + x^{2},\\
  f(\chi)&= \frac{1}{\chi^{2}-1}
  = \frac{4r^{2}r_{1}^{2}}{\rho_{+}^{2}\rho_{-}^{2}},\\
  \rho_{+}^{2}\rho_{-}^{2}f(\chi)
  &=
  4r^{2}r_{1}^{2},\\
  \frac{\partial^{k}}{\partial x^{k}}
  \left(\rho_{+}^{2}\rho_{-}^{2}f(\chi)\right)
  &=
  \sum_{q=0}^{k}\binom{k}{q}
  \frac{\partial^{q}}{\partial x^{q}}
  \left(\rho_{+}^{2}\rho_{-}^{2}\right)
  \frac{\partial^{k-q}f}{\partial x^{k-q}}
  = 
  \frac{\partial^{k}}{\partial x^{k}}\left(4r^{2}r_{1}^{2}\right),\\  
  \frac{\partial^{k}f}{\partial x^{k}}
  &=
  \frac{1}{\rho_{+}^{2}\rho_{-}^{2}}
  \left[
    \frac{\partial^{k}}{\partial x^{k}}\left(4r^{2}r_{1}^{2}\right)
    -
    \sum_{q=1}^{k}\binom{k}{q}
    \frac{\partial^{q}}{\partial x^{q}}
    \left(\rho_{+}^{2}\rho_{-}^{2}\right)
    \frac{\partial^{k-q}f}{\partial x^{k-q}}
  \right].\\
  \frac{\partial^{j+k}}{\partial r_{1}^{j}\partial x^{k}}
  \left[\rho_{+}^{2}\rho_{-}^{2}f(\chi)\right]
  &=
  \sum_{j,k}
  \binom{k}{q}
  \binom{j}{u}
  \frac{\partial^{u+q}}{\partial r_{1}^{u}\partial x^{q}}  
  \left(\rho_{+}^{2}\rho_{-}^{2}\right)
  \frac{\partial^{k+j-u-q} f}{\partial r_{1}^{j-u}\partial x^{k-q}}
  = 
  \frac{\partial^{j+k}}{\partial r_{1}^{j}\partial x^{k}}
  \left(4r^{2}r_{1}^{2}\right).
  % \frac{\partial}{\partial x}
\end{align*}

From Laplace equation:
\begin{align}
  \frac{1}{r}\frac{\partial}{\partial r}
  \left(
    \frac{\partial G_{n}}{\partial r}
  \right)
  +
  \frac{1}{r^{2}}\frac{\partial^{2}G_{n}}{\partial \theta^{2}}
  +
  \frac{\partial^{2}G_{n}}{\partial x^{2}} &= 0,\\
  \frac{\partial^{2}G_{n}}{\partial r^{2}}
  +
  \frac{1}{r}\frac{\partial G_{n}}{\partial r}
  -
  \frac{n^{2}}{r^{2}}G_{n}
  +
  \frac{\partial^{2}G_{n}}{\partial x^{2}}
  &= 0.
\end{align}

From Cohl, Rau, Tohline, et al.
\begin{align}
  G_{n}
  &=
  \frac{Q_{n-1/2}(\chi)}{2\pi\sqrt{rr_{1}}},\\
  &=
  \frac{(-1)^{n}}{2\sqrt{\rho\rho_{1}}}
    \sum_{i=0}^{\infty}
    \left(
      \frac{-1}{2}
    \right)^{i}
    \frac{(2i)!}{i!(2n+2i)!!}
    \left(
      \frac{\rho_{1}}{\rho}
    \right)^{n+2i+1/2}
    P_{n+2i}^{n}(\cos\phi),\\
    x &= \rho\cos\phi,\quad r = \rho\sin\phi,\\
    \rho_{1} &= r_{1}.
\end{align}

\begin{align}
  G_{n} &=
  \frac{Q_{n-1/2}(\chi)}{2\pi\sqrt{rr_{1}}},\\
  &=
  \sum_{q=0}^{\infty}
  \frac{1}{q!}\frac{\D^{q} Q_{n-1/2}(\chi_{0})}{\D \chi^{q}}
  \frac{(\chi-\chi_{0})^{q}}{\sqrt{r r_{1}}},\\
  \frac{(\chi - \chi_{0})^{q}}{\sqrt{rr_{1}}}
  &=
  \left[
    \frac{f(\delta r, \delta r_{1}, \delta x)}
    {4rr_{1}(r+\delta r)^{1/2}(r_{1}+\delta r_{1})^{1/2}}
  \right]^{q},\\
  f(\delta r, \delta r_{1}, \delta x)
  &=
  2rr_{1}
  \left[
    (r+\delta r)^{2} +
    (r_{1}+\delta r_{1})^{2} +
    (x+\delta x)^{2}
  \right]\nonumber\\
  &-
  2(r+\delta r)(r_{1}+\delta r_{1})
  (r^{2} + r_{1}^{2} + x^{2}),\\
  f^{q}
  &=
  \sum \frac{1}{m!}
  \left.
    \frac{\partial^{m} f^{q}}{\partial (\delta r)^{m}}
  \right|_{\delta r=0}
  \left(\delta r\right)^{m}\,\text{(polynomial)},\\
  \frac{(\chi - \chi_{0})^{q}}{\sqrt{rr_{1}}}
  &=
  \sqrt{2}\frac{f^{q}}{(2rr_{1})^{2q+1/2}}
  \sum_{i=0}^{\infty}
  \sum_{j=0}^{\infty}
  a_{i}^{(q+1/2)}
  a_{j}^{(q+1/2)}
  \left(\frac{\delta r}{r}\right)^{i}
  \left(\frac{\delta r_{1}}{r_{1}}\right)^{j}
\end{align}

Derivatives of $f$:
\begin{align}
  \frac{\partial f}{\partial \delta r}
  &=
  4rr_{1}(r+\delta r) - 2(r_{1}+\delta r_{1})(r^{2}+r_{1}^{2}+x^{2}),\\
  &= 4r^{2}r_{1} - 2r_{1}(r^{2}+r_{1}^{2}+x^{2}),\,\mathbf{\delta}=0,\\
  \frac{\partial^{2} f}{\partial (\delta r)^{2}}
  &=
  4rr_{1},\\
  \frac{\partial f^{q}}{\partial \delta r}
  &=
  qf^{q-1}\frac{\partial f}{\partial \delta r},\\
  \frac{\partial^{M} f^{q}}{\partial (\delta r)^{M}}
  &=
  q\sum_{m=0}^{M-1}
  \binom{M-1}{m}
  \frac{\partial^{m+1} f}{\partial (\delta r)^{m+1}}
  \frac{\partial^{M-m-1}f^{q-1}}{\partial (\delta r)^{M-m-1}}
\end{align}

\begin{align}
  \chi - \chi_{0}
  &=
  \frac{1}{2}\frac{f(\delta r, \delta r_{1}, \delta x)}{(r+\delta
    r)(r_{1}+\delta r_{1})},\\
  f(\delta r, \delta r_{1}, \delta x)
  &=
  A(\delta r) + B(\delta r_{1}) +  C(\delta r, \delta r_{1})
  + D(\delta x),\\
  A(\delta r) &=
  \left(\delta r\right)^{2} -
  \left(r_{1}^{2} - r^{2} + x^{2}\right)\frac{\delta r}{r}
  =
  \left(\delta r\right)^{2} + a\delta r,\\
  B(\delta r_{1}) &=
  \left(\delta r_{1}\right)^{2} -
  \left(r^{2} - r_{1}^{2} + x^{2}\right)\frac{\delta r_{1}}{r_{1}}
    =
  \left(\delta r_{1}\right)^{2} + b\delta r_{1},\\
  C(\delta r, \delta r_{1})
  &=
  -\frac{(r^{2} + r_{1}^{2} + x^{2})}{rr_{1}}\delta r \delta r_{1}
  =
  c\delta r\delta r_{1},
  \\
  D(\delta x)
  &=
  \left(\delta x\right)^{2} + 2x\delta x
  =
  d_{2}\left(\delta x\right)^{2} + d\delta x.  
\end{align}

\begin{align}
  \left[
    f(\delta r, \delta r_{1}, \delta x)
  \right]^{q}
  &=
  \sum_{|\bA|=q}\binom{q}{\bA}
  c^{\alpha_{3}}\nonumber\\
  &\times
  \left[\sum_{\beta=0}^{\alpha_{1}}
    \binom{\alpha_{1}}{\beta_{1}}
    %a_{2}^{\beta_{1}}
    a^{\alpha_{1}-\beta_{1}}
    \left(\delta r\right)^{\alpha_{1}+\alpha_{3}+\beta_{1}}
  \right]\nonumber\\
  &\times
  \left[\sum_{\beta_{2}=0}^{\alpha_{2}}
    \binom{\alpha_{2}}{\beta_{2}}
    %b_{2}^{\beta_{2}}
    b^{\alpha_{2}-\beta_{2}}
    \left(\delta r_{1}\right)^{\alpha_{2}+\alpha_{3}+\beta_{2}}
  \right]\nonumber\\
  &\times
  \left[\sum_{\beta_{4}=0}^{\alpha_{4}}
    \binom{\alpha_{4}}{\beta_{4}}
    % d_{2}^{\beta_{4}}
    d^{\alpha_{4}-\beta_{4}}
    \left(\delta x\right)^{\alpha_{4}+\beta_{4}}
  \right],\\
  &=
  \sum_{|\bA|=q}
  \frac{q!}{\alpha_{3}!}
  c^{\alpha_{3}}\nonumber\\
  &\times
  \left[\sum_{\beta_{1}=0}^{\alpha_{1}}
    % \frac{a_{2}^{\beta_{1}}a_{1}^{\alpha_{1}-\beta_{1}}}
    \frac{a^{\alpha_{1}-\beta_{1}}}
    {\beta_{1}!(\alpha_{1}-\beta_{1})!}
    \left(\delta r\right)^{\alpha_{1}+\alpha_{3}+\beta_{1}}
  \right]\nonumber\\
  &\times
  \left[\sum_{\beta_{2}=0}^{\alpha_{2}}
    %\frac{b_{2}^{\beta_{2}}b^{\alpha_{2}-\beta_{2}}}
    \frac{b^{\alpha_{2}-\beta_{2}}}
    {\beta_{2}!(\alpha_{2}-\beta_{2})!}
    \left(\delta r_{1}\right)^{\alpha_{2}+\alpha_{3}+\beta_{2}}
  \right]\nonumber\\
  &\times
  \left[\sum_{\beta_{4}=0}^{\alpha_{4}}
    %\binom{\alpha_{4}}{\beta_{4}}
    %\frac{d_{2}^{\beta_{4}}d^{\alpha_{4}-\beta_{4}}}
    \frac{d^{\alpha_{4}-\beta_{4}}}
    {\beta_{4}!(\alpha_{4}-\beta_{4})!}
    \left(\delta x\right)^{\alpha_{4}+\beta_{4}}
  \right].  
\end{align}

From Cohl, Rau, Tohline, Browne, Cazes, Barnes, 2001:
\begin{align}
  G_{n}
  &=
  \frac{1}{2\rho_{>}}
  \sum_{\ell=n}^{\infty}
  \frac{(\ell-n)!}{(\ell+n)!}
  \left(
    \frac{\rho_{<}}{\rho_{>}}
  \right)^{\ell}
  P_{\ell}^{n}(\cos\phi)
  P_{\ell}^{n}(\cos\phi_{1}),\\
  r &= \rho\sin\phi,\, z = \rho\cos\phi.
\end{align}

\begin{align}
  G_{n}^{m}
  &=
  \int_{0}^{2\pi}
  \frac{\cos n\theta_{1}}{4\pi R^{m}}\,\D \theta_{1},\\
  R^{2} &= r^{2} + r_{1}^{2} + z^{2} - 2rr_{1}\cos\theta_{1},\\
  G_{n}^{m}
  &=
  \frac{1}{2\pi\rho^{m}}
  \int_{0}^{\pi}
  \frac{\cos 2n\theta_{1}}{(1 - \lambda^{2}\cos^{2}\theta_{1})^{m/2}}
  \,\D\theta_{1},\\
  \rho^{2} &= (r+r_{1})^{2} + z^{2},\,
  \lambda^{2} = \frac{4rr_{1}}{\rho^{2}},\\
  G_{n}^{m}
  &=
  \frac{(-1)^{n}}{4\pi(\rho_{+}\rho_{-})^{m/2}}
  \int_{0}^{2\pi}
  \frac{\cos n\theta_{1}}{(\chi + \sqrt{\chi^{2}-1}\cos\theta_{1})^{m/2}}
  \,\D\theta_{1},\\
  \chi &=
  \frac{1}{2}\frac{\rho_{+}^{2}+\rho_{-}^{2}}{\rho_{+}\rho_{-}},\\
  G_{n}^{m}
  &=
  \frac{1}{2(\rho_{+}\rho_{-})^{m/2}}
  \frac{\Gamma(m/2-n)}{\Gamma(m/2)}
  P_{m/2-1}^{n}(\chi).
\end{align}

\begin{align}
  G_{0}^{1} &= \frac{K(\lambda)}{\pi\rho},\\
  G_{1}^{1} &=
  \frac{1}{\pi\rho}
  \left[
    2
    \frac{K(\lambda) - E(\lambda)}{\lambda^{2}}
    -
    K(\lambda)
  \right].
\end{align}

From DLMF~14.10.6 and~14.10.3
\begin{align}
  (m-2n-4)G_{n+2}^{m} +
  4(n+1)\frac{\chi}{\sqrt{\chi^{2}-1}}G_{n+1}^{m} -
  (m+2n)G_{n}^{m} &= 0,\\
  m(m+2)(\rho_{+}\rho_{-})^{2}G_{n}^{m+4}
  -2m(m+1)(\rho_{+}\rho_{-})\chi G_{n}^{m+2}
  +(m+2n)(m-2n)G_{n}^{m} &= 0.
\end{align}

Using G\&R~8.732,
\begin{align}
  \frac{\partial G_{n}}{\partial z}
  &=
  \frac{n+1/2}{\chi^{2}-1}
  \left(
    G_{n+1} - \chi G_{n}
  \right)\frac{z}{rr_{1}},\\
  &=
  (n+1/2)
  \left(
    F_{1}G_{n+1} - F_{2}G_{n}
  \right),\\
  F_{1} &= \frac{4rr_{1}z}{\rho_{+}^{2}\rho_{-}^{2}},\,
  F_{2} = 2z\frac{r^{2} + r_{1}^{2} + z^{2}}{\rho_{+}^{2}\rho_{-}^{2}}.
\end{align}

Higher derivatives:
\begin{align}
  \frac{\partial^{k+1} G_{n}}{\partial z^{k+1}}
  &=
  (n+1/2)
  \sum_{q=0}^{k}
  \binom{k}{q}
  \left(
    \frac{\partial^{k-q}F_{1}}{\partial z^{k-q}}
    \frac{\partial^{q} G_{n+1}}{\partial z^{q}}
    -
    \frac{\partial^{k-q}F_{2}}{\partial z^{k-q}}
    \frac{\partial^{q} G_{n}}{\partial z^{q}}    
  \right).
\end{align}


\begin{align}
  \frac{\partial G_{n}}{\partial r}
  &=
  -\frac{G_{n}}{2r}
  + (n+1/2)
  \left(
    A_{1}G_{n+1} -A_{2}G_{n}
  \right),\\
  A_{1}
  &=
  \frac{2r_{1}}{\rho_{+}^{2}\rho_{-}^{2}}
  \left(
    r^{2} - r_{1}^{2} - z^{2}
  \right),\,
  A_{2}
  =
  \frac{1}{r}\frac{1}{\rho_{+}^{2}\rho_{-}^{2}}
  \left[
    r^{4} - (r_{1}^{2}+z^{2})^{2}
  \right].
\end{align}

Generation of derivatives from Laplace equation:
\begin{align}
  \frac{\partial^{i+k+2}G_{n}}{\partial r^{i+2}\partial x^{k}}
    &=
    -\frac{\partial^{i+k+2} G_{n}}{\partial r^{i} \partial x^{k+2}}
    +
    n^{2}
    \sum_{u=0}^{i}
    (-1)^u \binom{i}{u} \frac{(u+1)!}{r^{u+2}}
    \frac{\partial^{i+k-u} G_{n}}{\partial r^{i-u}\partial x^{k}}\nonumber\\
    &-
    \sum_{u=0}^{i}
    (-1)^u \binom{i}{u} \frac{u!}{r^{u+1}}
    \frac{\partial^{i+k-u+1} G_{n}}{\partial r^{i-u+1}\partial x^{k}}.
\end{align}

\begin{align}
  % \frac{\partial G_{n}}{\partial x}
  % &=
  % (n-1/2)
  % \left(
  %   F_{1}G_{n} - F_{2}G_{n-1}
  % \right)x,\\
  % F_{1}
  % &=
  % \frac{\rho_{+}^{2}+\rho_{-}^{2}}{\rho_{+}^{2}\rho_{-}^{2}},\,
  % F_{2}
  % =
  % \frac{\rho_{+}^{2}-\rho_{-}^{2}}{\rho_{+}^{2}\rho_{-}^{2}}.\\
  \frac{\partial G_{n}}{\partial x}
  &=
  (n-1/2)
  \left[
    \frac{x}{\rho_{+}^{2}}(G_{n} + G_{n-1})
    +
    \frac{x}{\rho_{-}^{2}}(G_{n} - G_{n-1})
  \right],\\
  \frac{\partial^{k+1}G_{n}}{\partial x^{k+1}}
  &=
  (n-1/2)
  \sum_{q=0}^{k}
  \binom{k}{q}
  \left[
    \frac{\partial^{q}}{\partial x^{q}}
    \left(
      \frac{x}{\rho_{+}^{2}}
    \right)
    \frac{\partial^{k-q}}{\partial x^{k-q}}
    \left(G_{n}+G_{n-1}\right)
    +
    \frac{\partial^{q}}{\partial x^{q}}
    \left(
      \frac{x}{\rho_{-}^{2}}
    \right)
    \frac{\partial^{k-q}}{\partial x^{k-q}}
    \left(G_{n}-G_{n-1}\right)
  \right].
\end{align}

\begin{align}
  \frac{\partial G_{n}}{\partial r}
  &=
  -\frac{G_{n}}{2r}
  + (n-1/2)\frac{r^{2} - r_{1}^{2} - x^{2}}{2r}
  \left[
    \frac{1}{\rho_{+}^{2}}(G_{n} + G_{n-1})
    +
    \frac{1}{\rho_{-}^{2}}(G_{n} - G_{n-1})
  \right],\\
  \gnijk{n}{1}{0}{k}
  &=
  -\frac{\gnijk{n}{0}{0}{k}}{2r}
  + \frac{n-1/2}{2r}
  \sum_{q=0}^{k}
  \binom{k}{q}
  \begin{aligned}[t]
     \bigg[
    &\left(\gnijk{n}{0}{0}{k-q} + \gnijk{n-1}{0}{0}{k-q}\right)
    \frac{\partial^{q}}{\partial x^{q}}
    \frac{f(r,r_{1},x)}{\rho_{+}^{2}} + \\
    &\left(\gnijk{n}{0}{0}{k-q} - \gnijk{n-1}{0}{0}{k-q}\right)
    \frac{\partial^{q}}{\partial x^{q}}
    \frac{f(r,r_{1},x)}{\rho_{-}^{2}}
    \bigg],
  \end{aligned}\\
  f(r,r_{1},x) &= r^{2} - r_{1}^{2} - x^{2}.
\end{align}

\begin{align}
  \gnijk{n}{1}{1}{k}
  &=
  -\frac{\gnijk{n}{0}{1}{k}}{2r}
  +\frac{n-1/2}{2r}
  \sum_{q=0}^{k}
  \binom{k}{q}
    \begin{aligned}[t]
      \biggl[
      &
      \left(\gnijk{n}{0}{0}{k-q} + \gnijk{n-1}{0}{0}{k-q}\right)
      \frac{\partial^{q+1}}{\partial r_{1}\partial x^{q}}
      \frac{f(r,r_{1},x)}{\rho_{+}^{2}}
      + \\
      &
      \left(\gnijk{n}{0}{1}{k-q} + \gnijk{n-1}{0}{1}{k-q}\right)
      \frac{\partial^{q}}{\partial x^{q}}
      \frac{f(r,r_{1},x)}{\rho_{+}^{2}}
      + \\
      &
      \left(\gnijk{n}{0}{0}{k-q} - \gnijk{n-1}{0}{0}{k-q}\right)
      \frac{\partial^{q+1}}{\partial r_{1}\partial x^{q}}
      \frac{f(r,r_{1},x)}{\rho_{-}^{2}}
      + \\
      &
      \left(\gnijk{n}{0}{1}{k-q} - \gnijk{n-1}{0}{1}{k-q}\right)
      \frac{\partial^{q}}{\partial x^{q}}
      \frac{f(r,r_{1},x)}{\rho_{-}^{2}}
      \biggr]
    \end{aligned}
\end{align}

\begin{align}
  \frac{\partial}{\partial x}
  \frac{x}{\rho_{\pm}^{2}}
  &=
  \left[
    1 - 2x\frac{x}{\rho_{\pm}^{2}}
  \right]
  \frac{1}{\rho_{\pm}^{2}},\\
  \frac{\partial^{n}}{\partial x^{n}}
  \frac{x}{\rho_{\pm}^{2}}
  &=
  -\frac{n}{\rho_{\pm}^{2}}
  \left[
    2x
    \frac{\partial^{n-1}}{\partial x^{n-1}}
    \frac{x}{\rho_{\pm}^{2}}
    +
    (n-1)
    \frac{\partial^{n-2}}{\partial x^{n-2}}
    \frac{x}{\rho_{\pm}^{2}}    
  \right],\,n\geq 2.
\end{align}

This bit can go in a paper.

Transfer operator:
\begin{align}
  G_{n}(r,r_{1},x)
  &=
  \sum_{m=0}^{\infty}
  \sum_{i+j+k=m}
  \gnbarijk{n}{i}{j}{k}(\Delta r)^{i}(\Delta r_{1})^{j}(\Delta
  x)^{k},\\
  \gnbarijk{n}{i}{j}{k}(r,r_{1},x)
  &=
  \frac{1}{i!j!k!}
  \frac{\partial^{i+j+k}}
  {\partial r^{i}\partial r_{1}^{j}\partial x^{k}}
  G_{n}(r,r_{1},x).
\end{align}

Source expansion, for $M$ point sources:
\begin{align}
  S_{ij} &= \sum_{m=1}^{M}\sigma^{(m)}
  (\Delta r_{1}^{(m)})^{i}(\Delta z_{1}^{(m)})^{j}
\end{align}

\begin{align}
  \phi(r,z)
  &=
  \sum_{i,j} (-1)^{j}S_{ij}\gnbarijk{n}{0}{i}{j}(r,r_{1},z-z_{1}),\\
  \phi(r+\Delta r, z+\Delta z)
  &=
  \sum_{k,\ell}\Phi_{k\ell}
  (\Delta r)^{k}(\Delta z)^{\ell},\\
  \Phi_{k\ell}
  &=
  \sum_{i,j}
  (-1)^{j}
  \binom{j+\ell}{j}
  s_{ij}\gnbarijk{n}{k}{i}{j+\ell}(r,r_{1},z-z_{1})
\end{align}

Moment and expansion shifting from $(r,z)$ to $(r+\Delta r, z+\Delta
r)$ (primes indicate original centre of moment or expansion),
\begin{align}
  S_{ij}
  &=
  \sum_{q=0}^{i}
  \sum_{u=0}^{j}
  \binom{i}{q}
  \binom{j}{u}
  (-\Delta r_{1})^{q}
  (-\Delta z_{1})^{u}
  S_{i-q,j-u}',\\
  \Phi_{ij}
  &=
  \sum_{q=0}^{\infty}
  \sum_{u=0}^{\infty}
  \binom{i+q}{q}
  \binom{j+u}{u}
  (-\Delta r)^{q}
  (-\Delta z)^{u}
  \Phi_{i+q,j+u}'.  
\end{align}

For ``backward'' translation (switching $z$ and $z_{1}$), use the same
derivatives of $G$ and change the signs of $\Delta z$ and $\Delta
z_{1}$:
\begin{align}
  \phi(r+\Delta r, z_{1}+\Delta z)
  &=
  \sum_{k,\ell}
  (-1)^{\ell}
  (\Delta r)^{k}(\Delta z)^{\ell}
  \sum_{i,j}
  % (-1)^{j}
  S_{ij}\gnbarijk{n}{k}{i}{j+l}(r,r_{1},z-z_{1}).  
\end{align}

For ``inward'' translation (switching $r$ and $r_{1}$), switch indices
in derivatives of $G$,
\begin{align}
  \Phi_{k\ell}
  &=
  \sum_{i,j}
  (-1)^{j}s_{ij}\gnbarijk{n}{i}{k}{j+\ell}(r,r_{1},z-z_{1})
\end{align}

Separation of boxes. For box at radial station $i$, boxes at radial
stations $j$ are well separated, if:
\begin{align*}
  j \geq \left[\chi + \left(\chi^{2}-1\right)^{1/2}\right](i+1).
\end{align*}

Boxes with axial displacement $j$ are well separated if
\begin{align*}
  j \geq \sqrt{2}\left(\chi-1\right)^{1/2}(i+1).
\end{align*}

\end{document}

%%% Local Variables:
%%% mode: latex
%%% TeX-master: t
%%% End:
